Finished transitioning all proofs from coq

formalization/Formalization/Syntax.lean
@@ -26,7 +26,14 @@ inductive Exp where
   | rproj  : Exp → String → Exp
   deriving Repr
 
-inductive IndexLookup : Typ -> Nat → Typ → Prop 
+inductive Value : Exp → Prop
+| vint  : ∀ n, Value (Exp.lit n)
+| vunit : Value unit
+| vclos : ∀ v A e, Value v → Value (Exp.clos v A e)
+| vrcd  : ∀ l v, Value v → Value (Exp.lrec l v)
+| vmrg  : ∀ v₁ v₂, Value v₁ → Value v₂ → Value (Exp.binop Op.mrg v₁ v₂) 
+
+inductive IndexLookup : Typ -> Nat-> Typ -> Prop 
 | zero (A B : Typ) : IndexLookup (Typ.and A B) 0 B
 | succ (A B : Typ) (n : Nat) (C : Typ) : IndexLookup A n C → IndexLookup (Typ.and A B) (Nat.succ n) C
 
@@ -34,6 +41,54 @@ inductive LabelIn : String -> Typ -> Prop
 | rcd (label : String) (T : Typ) : LabelIn label (Typ.rcd label T)
 | andl (A B : Typ) (label : String) : LabelIn label A → LabelIn label (Typ.and A B)
 | andr (A B : Typ) (label : String) : LabelIn label B → LabelIn label (Typ.and A B)
+
+inductive RecordLookup : Typ → String → Typ → Prop
+| zero (label : String) (T : Typ) :
+    RecordLookup (Typ.rcd label T) label T
+| andl (A B : Typ) (label : String) (T : Typ) :
+    RecordLookup A label T →
+    LabelIn label A ∧ ¬ LabelIn label B →
+    RecordLookup (Typ.and A B) label T
+| andr (A B : Typ) (label : String) (T : Typ) :
+    RecordLookup B label T →
+    LabelIn label B ∧ ¬ LabelIn label A →
+    RecordLookup (Typ.and A B) label T
+
+inductive HasType : Typ -> Exp -> Typ -> Prop
+| ctx (EnvT : Typ) : HasType EnvT Exp.ctx EnvT
+| int (EnvT : Typ) (i : Nat) : HasType EnvT (Exp.lit i) Typ.int
+| unit (EnvT : Typ) : HasType EnvT Exp.unit Typ.top
+| app (EnvT A B : Typ) (e1 e2 : Exp) :
+    HasType EnvT e1 (Typ.arr A B) →
+    HasType EnvT e2 A →
+    HasType EnvT (Exp.binop Op.app e1 e2) B
+| box (EnvT EnvT₁ A: Typ) (e1 e2 : Exp) :
+    HasType EnvT e1 EnvT₁ →
+    HasType EnvT₁ e2 A →
+    HasType EnvT (Exp.binop Op.box e1 e2) A
+| mrg (EnvT A B: Typ) (e1 e2 : Exp) :
+    HasType EnvT e1 A →
+    HasType (Typ.and EnvT A) e2 B →
+    HasType EnvT (Exp.binop Op.mrg e1 e2) (Typ.and A B)
+| lam (EnvT A B : Typ) (e : Exp) :
+    HasType (Typ.and EnvT A) e B →
+    HasType EnvT (Exp.lam A e) (Typ.arr A B)
+| proj (EnvT A B : Typ) (e : Exp) (n : Nat) :
+    HasType EnvT e A →
+    IndexLookup A n B →
+    HasType EnvT (Exp.proj e n) B
+| clos (EnvT EnvT₁ A B : Typ) (e env : Exp) : 
+    Value env →
+    HasType Typ.top env EnvT₁ →
+    HasType (Typ.and EnvT₁ A) e B →
+    HasType EnvT (Exp.clos env A e) (Typ.arr A B)
+| rcd (EnvT A : Typ) (e : Exp) (label : String) :
+    HasType EnvT e A →
+    HasType EnvT (Exp.lrec label e) (Typ.rcd label A)
+| rproj (EnvT A B : Typ) (e : Exp) (label : String) :
+    HasType EnvT e B →
+    RecordLookup B label A →
+    HasType EnvT (Exp.rproj e label) A 
 
 end LambdaE
 
@@ -75,6 +130,23 @@ inductive IndexLookup : Typ → Nat → Typ → Prop
 | zero (A B : Typ) : IndexLookup (Typ.and A B) 0 B
 | succ (A B : Typ) (n : Nat) (C : Typ) : IndexLookup A n C → IndexLookup (Typ.and A B) (Nat.succ n) C
 
+inductive LabelIn : String -> Typ -> Prop
+| rcd (label : String) (T : Typ) : LabelIn label (Typ.rcd label T)
+| andl (A B : Typ) (label : String) : LabelIn label A → LabelIn label (Typ.and A B)
+| andr (A B : Typ) (label : String) : LabelIn label B → LabelIn label (Typ.and A B)
+
+inductive RecordLookup : Typ → String → Typ → Prop
+| zero (label : String) (T : Typ) :
+    RecordLookup (Typ.rcd label T) label T
+| andl (A B : Typ) (label : String) (T : Typ) :
+    RecordLookup A label T →
+    LabelIn label A ∧ ¬ LabelIn label B →
+    RecordLookup (Typ.and A B) label T
+| andr (A B : Typ) (label : String) (T : Typ) :
+    RecordLookup B label T →
+    LabelIn label B ∧ ¬ LabelIn label A →
+    RecordLookup (Typ.and A B) label T
+
 def ElaborateType : Typ → LambdaE.Typ
   | Typ.int        => LambdaE.Typ.int
   | Typ.top        => LambdaE.Typ.top
@@ -83,24 +155,93 @@ def ElaborateType : Typ → LambdaE.Typ
   | Typ.rcd str t  => LambdaE.Typ.rcd str (ElaborateType t)
   | Typ.sig t1 t2  => LambdaE.Typ.arr (ElaborateType t1) (ElaborateType t2)
 
-inductive LabelIn : String -> Typ -> Prop
-| rcd (label : String) (T : Typ) : LabelIn label (Typ.rcd label T)
-| andl (A B : Typ) (label : String) : LabelIn label A → LabelIn label (Typ.and A B)
-| andr (A B : Typ) (label : String) : LabelIn label B → LabelIn label (Typ.and A B)
+inductive ElaborateExp : Typ -> Exp -> Typ -> LambdaE.Exp -> Prop
+| ctx (EnvT : Typ) : ElaborateExp EnvT Exp.ctx EnvT LambdaE.Exp.ctx
+| int (EnvT : Typ) (i : Nat) : ElaborateExp EnvT (Exp.lit i) Typ.int (LambdaE.Exp.lit i)
+| unit (EnvT : Typ) : ElaborateExp EnvT Exp.unit Typ.top LambdaE.Exp.unit
+| proj (EnvT A B : Typ) (n : Nat) (e : Exp) (ce : LambdaE.Exp) :
+    ElaborateExp EnvT e A ce →
+    IndexLookup A n B →
+    ElaborateExp EnvT (Exp.proj e n) B (LambdaE.Exp.proj ce n)
+| lam (EnvT A B : Typ) (e : Exp) (ce : LambdaE.Exp) :
+    ElaborateExp (Typ.and EnvT A) e B ce →
+    ElaborateExp EnvT (Exp.lam A e) (Typ.arr A B) (LambdaE.Exp.lam (ElaborateType A) ce)
+| box (EnvT EnvT₁ A: Typ) (e₁ e₂ : Exp) (ce₁ ce₂ : LambdaE.Exp) :
+    ElaborateExp EnvT e₁ EnvT₁ ce₁ →
+    ElaborateExp EnvT₁ e₂ A ce₂ →
+    ElaborateExp EnvT (Exp.binop Op.withE e₁ e₂) A
+    (LambdaE.Exp.binop LambdaE.Op.box ce₁ ce₂)
+| clos (EnvT EnvT₁ A B : Typ) (e env : Exp) (ce cenv : LambdaE.Exp) :
+    ElaborateExp EnvT env EnvT₁ cenv →
+    ElaborateExp (Typ.and EnvT₁ A) e B ce →
+    ElaborateExp EnvT (Exp.clos env A e) (Typ.arr A B) 
+    (LambdaE.Exp.binop LambdaE.Op.box cenv (LambdaE.Exp.lam (ElaborateType A) ce))
+| app (EnvT A B : Typ) (e₁ e₂ : Exp) (ce₁ ce₂ : LambdaE.Exp) :
+    ElaborateExp EnvT e₁ (Typ.arr A B) ce₁ →
+    ElaborateExp EnvT e₂ A ce₂ →
+    ElaborateExp EnvT (Exp.binop Op.app e₁ e₂) B
+    (LambdaE.Exp.binop LambdaE.Op.app ce₁ ce₂)
+| dmrg (EnvT A B : Typ) (e₁ e₂ : Exp) (ce₁ ce₂ : LambdaE.Exp) :
+    ElaborateExp EnvT e₁ A ce₁ →
+    ElaborateExp (Typ.and EnvT A) e₂ B ce₂ →
+    ElaborateExp EnvT (Exp.binop Op.dmrg e₁ e₂) (Typ.and A B)
+    (LambdaE.Exp.binop LambdaE.Op.mrg ce₁ ce₂)
+| ndmrg (EnvT A B : Typ) (e₁ e₂ : Exp) (ce₁ ce₂ : LambdaE.Exp) :
+    ElaborateExp EnvT e₁ A ce₁ →
+    ElaborateExp EnvT e₂ B ce₂ →
+    ElaborateExp EnvT (Exp.binop Op.ndmrg e₁ e₂) (Typ.and A B)
+    (LambdaE.Exp.binop LambdaE.Op.app
+      (LambdaE.Exp.lam (ElaborateType EnvT)
+        (LambdaE.Exp.binop LambdaE.Op.mrg
+          (LambdaE.Exp.binop LambdaE.Op.box (LambdaE.Exp.proj LambdaE.Exp.ctx 0) ce₁)
+          (LambdaE.Exp.binop LambdaE.Op.box (LambdaE.Exp.proj LambdaE.Exp.ctx 1) ce₂)))
+      LambdaE.Exp.ctx)
+| struct (EnvT A B : Typ) (e : Exp) (ce : LambdaE.Exp) :
+    ElaborateExp (Typ.and Typ.top A) e B ce →
+    ElaborateExp EnvT (Exp.struct A e) (Typ.sig A B) (LambdaE.Exp.binop LambdaE.Op.box LambdaE.Exp.unit (LambdaE.Exp.lam (ElaborateType A) ce))
+| modapp (EnvT A B : Typ) (e₁ e₂ : Exp) (ce₁ ce₂ : LambdaE.Exp) :
+    ElaborateExp EnvT e₁ (Typ.sig A B) ce₁ →
+    ElaborateExp EnvT e₂ A ce₂ →
+    ElaborateExp EnvT (Exp.binop Op.mapp e₁ e₂) B
+    (LambdaE.Exp.binop LambdaE.Op.app ce₁ ce₂)
+| lrec (EnvT A : Typ) (e : Exp) (ce : LambdaE.Exp) (label : String) :
+    ElaborateExp EnvT e A ce →
+    ElaborateExp EnvT (Exp.lrec label e) (Typ.rcd label A)
+    (LambdaE.Exp.lrec label ce)
+| rproj (EnvT A B : Typ) (e : Exp) (ce : LambdaE.Exp) (label : String) :
+    ElaborateExp EnvT e B ce →
+    RecordLookup B label A →
+    ElaborateExp EnvT (Exp.rproj e label) A (LambdaE.Exp.rproj ce label)
+| slet (EnvT A B : Typ) (e₁ e₂ : Exp) (ce₁ ce₂ : LambdaE.Exp) :
+    ElaborateExp EnvT e₁ A ce₁ →
+    ElaborateExp (Typ.and EnvT A) e₂ B ce₂ →
+    ElaborateExp EnvT (Exp.slet e₁ A e₂) B
+    (LambdaE.Exp.binop LambdaE.Op.app
+      (LambdaE.Exp.lam (ElaborateType A) ce₂)
+      ce₁)
+| sopen (EnvT A B : Typ) (e₁ e₂ : Exp) (ce₁ ce₂ : LambdaE.Exp) (label : String) :
+    RecordLookup (Typ.rcd label A) label B →
+    ElaborateExp EnvT e₁ (Typ.rcd label A) ce₁ →
+    ElaborateExp EnvT (Exp.rproj e₁ label) A (LambdaE.Exp.rproj ce₁ label) →
+    ElaborateExp (Typ.and EnvT A) e₂ B ce₂ →
+    ElaborateExp EnvT (Exp.sopen e₁ e₂) B
+    (LambdaE.Exp.binop LambdaE.Op.app
+      (LambdaE.Exp.lam (ElaborateType A) ce₂)
+      (LambdaE.Exp.rproj ce₁ label))
 end ENVCAP
 
-theorem TypeElaborationUniqueness : ∀ (srcT : ENVCAP.Typ) (dstT1 dstT2 : LambdaE.Typ),
-    ENVCAP.ElaborateType srcT = dstT1 →
-    ENVCAP.ElaborateType srcT = dstT2 →
-    dstT1 = dstT2 := by 
-  intro srcT dstT1 dstT2 h1 h2;
+theorem TypeElaborationUniqueness : ∀ (ST : ENVCAP.Typ) (CT₁ CT₂ : LambdaE.Typ),
+    ENVCAP.ElaborateType ST = CT₁ →
+    ENVCAP.ElaborateType ST = CT₂ →
+    CT₁ = CT₂ := by 
+  intro ST CT₁ CT₂ h1 h2;
   rw [← h1];
   rw [← h2];
 
-theorem TypeSafeIndexLookup : ∀ (srcT1 : ENVCAP.Typ) (n : Nat) (srcT2 : ENVCAP.Typ),
-    ENVCAP.IndexLookup srcT1 n srcT2 → 
-    LambdaE.IndexLookup (ENVCAP.ElaborateType srcT1) n (ENVCAP.ElaborateType srcT2) := by
-      intro srcT1 n srcT2 H;
+theorem TypeSafeIndexLookup : ∀ (ST₁ ST₂ : ENVCAP.Typ) (n : Nat), 
+    ENVCAP.IndexLookup ST₁ n ST₂ → 
+    LambdaE.IndexLookup (ENVCAP.ElaborateType ST₁) n (ENVCAP.ElaborateType ST₂) := by
+      intro ST₁ n ST₂ H;
       induction H with
       | zero A B =>
           apply LambdaE.IndexLookup.zero;
@@ -109,10 +250,10 @@ theorem TypeSafeIndexLookup : ∀ (srcT1 : ENVCAP.Typ) (n : Nat) (srcT2 : ENVCAP
           apply LambdaE.IndexLookup.succ;  
           apply IH;
         
-theorem TypeSafeLabelIn : ∀ (label : String) (srcT : ENVCAP.Typ),
-    ENVCAP.LabelIn label srcT ↔ 
-    LambdaE.LabelIn label (ENVCAP.ElaborateType srcT) := by
-      intro label srcT;
+theorem TypeSafeLabelExistence: ∀ (label : String) (ST : ENVCAP.Typ),
+    ENVCAP.LabelIn label ST ↔ 
+    LambdaE.LabelIn label (ENVCAP.ElaborateType ST) := by
+      intro label ST;
       apply Iff.intro;
       · intro H;
         induction H with
@@ -128,7 +269,7 @@ theorem TypeSafeLabelIn : ∀ (label : String) (srcT : ENVCAP.Typ),
             apply LambdaE.LabelIn.andr;
             apply IH;
       · intro H;
-        induction srcT with
+        induction ST with
         | rcd labelA T IH => 
             rw [ENVCAP.ElaborateType] at H;
             cases H
@@ -145,3 +286,394 @@ theorem TypeSafeLabelIn : ∀ (label : String) (srcT : ENVCAP.Typ),
                 apply IH2;
                 apply H2;
         | _ => cases H
+
+theorem TypeSafeLabelNonExistence : ∀ (label : String) (ST : ENVCAP.Typ),
+    ¬ ENVCAP.LabelIn label ST ↔ 
+    ¬ LambdaE.LabelIn label (ENVCAP.ElaborateType ST) := by
+      intro label ST;
+      apply Iff.intro;
+      · intro H1 H2;
+        have H3 := TypeSafeLabelExistence label ST;
+        apply H1;
+        apply H3.mpr;
+        apply H2;
+      · intro H1 H2;
+        have H3 := TypeSafeLabelExistence label ST;
+        apply H1;
+        apply H3.mp;
+        apply H2;
+
+theorem TypeSafeRecordLookup : ∀ (ST₁ ST₂: ENVCAP.Typ) (label : String),  
+    ENVCAP.RecordLookup ST₁ label ST₂ → 
+    LambdaE.RecordLookup (ENVCAP.ElaborateType ST₁) label (ENVCAP.ElaborateType ST₂) := by
+      intro ST₁ label ST₂ H;
+      induction H with
+      | zero label T =>
+          apply LambdaE.RecordLookup.zero;
+      | andl A B label T H1 H2 IH =>
+          rw [ENVCAP.ElaborateType];
+          apply LambdaE.RecordLookup.andl;
+          · apply IH;
+          · apply And.intro
+            · rw [← TypeSafeLabelExistence label A];
+              apply H2.left;
+            · rw [← TypeSafeLabelNonExistence label B];
+              apply H2.right;
+      | andr A B label T H1 H2 IH =>
+          rw [ENVCAP.ElaborateType];
+          apply LambdaE.RecordLookup.andr;
+          · apply IH;
+          · apply And.intro
+            · rw [← TypeSafeLabelExistence label B];
+              apply H2.left;
+            · rw [← TypeSafeLabelNonExistence label A];
+              apply H2.right;
+
+theorem TypePreservation : ∀ (EnvT ST : ENVCAP.Typ) (e : ENVCAP.Exp) (CT : LambdaE.Typ) (ce : LambdaE.Exp),
+    ENVCAP.ElaborateExp EnvT e ST ce →
+    LambdaE.HasType (ENVCAP.ElaborateType EnvT) ce (ENVCAP.ElaborateType ST) := by
+      intro EnvT ST e CT ce H;
+      induction H with
+      | ctx EnvT => apply LambdaE.HasType.ctx;
+      | int EnvT n => apply LambdaE.HasType.int;
+      | unit EnvT => apply LambdaE.HasType.unit;
+      | proj EnvT A B n e ce H1 H2 IH =>
+          apply LambdaE.HasType.proj; 
+          · apply IH;
+          · apply TypeSafeIndexLookup;
+            apply H2;
+      | lam EnvT A B e ce H IH => 
+          apply LambdaE.HasType.lam;
+          apply IH;
+      | box EnvT EnvT₁ A e₁ e₂ ce₁ ce₂ H1 H2 IH1 IH2 => 
+          apply LambdaE.HasType.box;
+          · apply IH1;
+          · apply IH2;
+      | clos EnvT EnvT₁ A B e env ce cenv H1 H2 IH1 IH2 => 
+          rw [ENVCAP.ElaborateType];
+          apply LambdaE.HasType.box;
+          · apply IH1;
+          · apply LambdaE.HasType.lam;
+            apply IH2;
+      | app EnvT A B e₁ e₂ ce₁ ce₂ H1 H2 IH1 IH2 =>
+          apply LambdaE.HasType.app;
+          · apply IH1;
+          · apply IH2;
+      | dmrg EnvT A B e₁ e₂ ce₁ ce₂ H1 H2 IH1 IH2 =>
+          apply LambdaE.HasType.mrg;
+          · apply IH1;
+          · apply IH2;
+      | ndmrg EnvT A B e₁ e₂ ce₁ ce₂ H1 H2 IH1 IH2 =>
+          apply LambdaE.HasType.app;
+          · apply LambdaE.HasType.lam;
+            apply LambdaE.HasType.mrg;
+            · apply LambdaE.HasType.box;
+              · apply LambdaE.HasType.proj;
+                · apply LambdaE.HasType.ctx;
+                · apply LambdaE.IndexLookup.zero;
+              · apply IH1;
+            · apply LambdaE.HasType.box;
+              · apply LambdaE.HasType.proj;
+                · apply LambdaE.HasType.ctx;
+                · apply LambdaE.IndexLookup.succ;
+                  · apply LambdaE.IndexLookup.zero;
+              · apply IH2;
+          · apply LambdaE.HasType.ctx;
+      | struct EnvT A B e ce H IH =>
+          apply LambdaE.HasType.box;
+          · apply LambdaE.HasType.unit;
+          · rw [ENVCAP.ElaborateType];
+            apply LambdaE.HasType.lam;
+            apply IH;
+      | modapp EnvT A B e₁ e₂ ce₁ ce₂ H1 H2 IH1 IH2 =>
+          apply LambdaE.HasType.app;
+          · apply IH1;
+          · apply IH2;
+      | lrec EnvT A e ce label H IH =>            
+          apply LambdaE.HasType.rcd;
+          apply IH;
+      | rproj EnvT A B e ce label H1 H2 IH =>
+          apply LambdaE.HasType.rproj;
+          · apply IH;
+          · apply TypeSafeRecordLookup;
+            apply H2;
+      | slet EnvT A B e₁ e₂ ce₁ ce₂ H1 H2 IH1 IH2 =>
+          apply LambdaE.HasType.app; 
+          · apply LambdaE.HasType.lam;
+            apply IH2;
+          · apply IH1;
+      | sopen EnvT A B e₁ e₂ ce₁ ce₂ label H1 H2 H3 IH1 IH2 IH3 IH4 =>
+          apply LambdaE.HasType.app; 
+          · apply LambdaE.HasType.lam;
+            apply IH4;
+          · apply LambdaE.HasType.rproj;
+            · apply IH2;
+            · apply TypeSafeRecordLookup;
+              apply ENVCAP.RecordLookup.zero
+
+theorem SlookupUniqueness : ∀ (EnvT T₁ T₂: ENVCAP.Typ) (n : Nat),
+    ENVCAP.IndexLookup EnvT n T₁ →
+    ENVCAP.IndexLookup EnvT n T₂ →
+    T₁ = T₂ := by
+      intro EnvT T₁ T₂ n H1 H2;
+      induction H1 with
+      | zero A B =>
+          cases H2;
+          rfl;
+      | succ A B n C H IH =>
+        apply IH;
+        cases H2 with
+        | succ _ _ _ _ h => exact h  
+
+theorem RLookupUniqueness : ∀ (RT T₁ T₂: ENVCAP.Typ) (label : String),
+    ENVCAP.RecordLookup RT label T₁ →
+    ENVCAP.RecordLookup RT label T₂ →
+    T₁ = T₂ := by
+      intro RT T₁ T₂ label H1 H2;
+      induction H1 with
+      | zero label T =>
+          cases H2;
+          rfl;
+      | andl A B label T H3 H4 IH =>
+        apply IH;
+        cases H2 with
+        | andl _ _ _ _ h1 h2 => apply h1
+        | andr _ _ _ _ h1 h2 => 
+          cases H4 with | intro ha hb =>
+          cases h2 with | intro hc hd =>
+          exfalso; apply hb; apply hc
+      | andr A B label T H3 H4 IH => 
+        apply IH;
+        cases H2 with
+        | andr _ _ _ _ h1 h2 => apply h1
+        | andl _ _ _ _ h1 h2 => 
+          cases H4 with | intro ha hb =>
+          cases h2 with | intro hc hd =>
+          exfalso; apply hb; apply hc
+
+theorem InferenceUniqueness : ∀ (EnvT T₁ T₂ : ENVCAP.Typ) (e : ENVCAP.Exp) (ce₁ ce₂ : LambdaE.Exp),
+    ENVCAP.ElaborateExp EnvT e T₁ ce₁ →
+    ENVCAP.ElaborateExp EnvT e T₂ ce₂ →
+    T₁ = T₂ := by
+      intro EnvT T₁ T₂ e ce₁ ce₂ H1 H2;
+      revert T₂;
+      revert ce₂;
+      induction H1 with
+      | ctx EnvT =>
+          intro ce₂ T₂ H2;
+          cases H2;
+          rfl;
+      | int EnvT n =>
+          intro ce₂ T₂ H2;
+          cases H2;
+          rfl;
+      | unit EnvT =>
+          intro ce₂ T₂ H2;
+          cases H2;
+          rfl;
+      | proj EnvT A B n e ce H1 H2 IH =>
+          intro ce₂ T₂ H3;
+          cases H3 with
+          | proj _ a' _ _ _ ce' H4 H5 =>
+              have hA : A = a' := by apply IH; apply H4;
+              rw [hA] at H2;
+              apply SlookupUniqueness a' B T₂ n;
+              · apply H2;
+              · apply H5;
+      | lam EnvT A B e ce H IH => 
+          intro ce₂ T₂ H2;
+          cases H2 with
+          | lam _ _ b' _ ce' h =>
+              have hA : B = b' := by apply IH; apply h;
+              rw [hA];
+      | box EnvT EnvT₁ A e₁ e₂ ce₁ ce₂ H1 H2 IH1 IH2 => 
+          intro ce' T' H3;
+          cases H3 with
+          | box _ en _ _ _ ce1' ce2' h1 h2 =>
+            have hA : EnvT₁ = en :=  by apply IH1; apply h1;
+            rw [hA] at IH2;
+            apply IH2;
+            apply h2;
+      | clos EnvT EnvT₁ A B e env ce cenv H1 H2 IH1 IH2 =>
+          intro ce' T' H3;
+          cases H3 with
+          | clos _ et _ bT _ _ ce1' cenv' h1 h2 =>
+            have hA : EnvT₁ = et := by apply IH1; apply h1;
+            have hB : B = bT := by apply IH2;  rw [hA]; apply h2;
+            rw [hB];
+      | app EnvT A B e₁ e₂ ce₁ ce₂ H1 H2 IH1 IH2 =>
+          intro ce' T' H3;
+          cases H3 with
+          | app _ a' _ _ _ ce1' ce2' h1 h2 =>
+            have hA : ENVCAP.Typ.arr A B = ENVCAP.Typ.arr a' T' := by apply IH1; apply h1;
+            cases hA;
+            rfl;
+      | dmrg EnvT A B e₁ e₂ ce₁ ce₂ H1 H2 IH1 IH2 =>
+          intro ce' T' H3;
+          cases H3 with
+          | dmrg _ a' b' _ _ ce1' ce2' h1 h2 =>
+            have hA : A = a' := by apply IH1; apply h1;
+            have hB : B = b' := by rw [hA] at IH2; apply IH2; apply h2;
+            rw [hA, hB];
+      | ndmrg EnvT A B e₁ e₂ ce₁ ce₂ H1 H2 IH1 IH2 =>
+          intro ce' T' H3;
+          cases H3 with
+          | ndmrg _ a' b' _ _ ce1' ce2' h1 h2 =>
+            have hA : A = a' := by apply IH1; apply h1;
+            have hB : B = b' := by apply IH2; apply h2;
+            rw [hA, hB];
+      | struct EnvT A B e ce H IH => 
+          intro ce' T' H2;
+          cases H2 with
+          | struct _ a' b' _ ce1' h =>
+              have hA : B = b' := by apply IH; apply h;
+              rw [hA];
+      | modapp EnvT A B e₁ e₂ ce₁ ce₂ H1 H2 IH1 IH2 =>
+          intro ce' T' H3;
+          cases H3 with
+          | modapp _ a' _ _ _ ce1' ce2' h1 h2 =>
+            have hA : A = a' := by apply IH2; apply h2;
+            have hB : ENVCAP.Typ.sig A B = ENVCAP.Typ.sig a' T' := by apply IH1; apply h1;
+            cases hB;
+            rfl;
+      | lrec EnvT A e ce label H IH => 
+          intro ce' T' H2;
+          cases H2 with
+          | lrec _ a' _ ce1' label h =>
+              have hA : A = a' := by apply IH; apply h;
+              rw [hA];
+      | rproj EnvT A B e ce label H1 H2 IH => 
+          intro ce' T' H3;
+          cases H3 with
+          | rproj _ a' b' _ ce1' _ h1 h2 =>
+            have hA : B = b' := by apply IH; apply h1;
+            apply RLookupUniqueness; 
+            · apply H2;
+            · rw [hA];
+              apply h2;
+      | slet EnvT A B e₁ e₂ ce₁ ce₂ H1 H2 IH1 IH2 =>
+          intro ce' T' H3;
+          cases H3 with
+          | slet _ _ b' _ _ ce1' ce2' h1 h2 =>
+            apply IH2;
+            apply h2;
+      | sopen EnvT A B e₁ e₂ ce₁ ce₂ label H1 H2 H3 IH1 IH2 IH3 IH4 =>
+          intro ce' T' H5;
+          cases H5 with
+          | sopen _ a' b' _ _ ce1' ce2' label' h1 h2 h3 h4 =>
+            have hA : ENVCAP.Typ.rcd label A = ENVCAP.Typ.rcd label' a' := by apply IH2; apply h2;
+            cases hA;
+            apply IH4;
+            apply h4;
+
+theorem ElaborationUniqueness : ∀ (EnvT T₁ T₂ : ENVCAP.Typ) (e : ENVCAP.Exp) (ce₁ ce₂ : LambdaE.Exp),
+    ENVCAP.ElaborateExp EnvT e T₁ ce₁ →
+    ENVCAP.ElaborateExp EnvT e T₂ ce₂ →
+    ce₁ = ce₂ := by
+      intro EnvT T₁ T₂ e ce₁ ce₂ H1 H2;
+      revert T₂;
+      revert ce₂;
+      induction H1 with
+      | ctx EnvT =>
+          intro ce₂ T₂ H2;
+          cases H2;
+          rfl;
+      | int EnvT n =>
+          intro ce₂ T₂ H2;
+          cases H2;
+          rfl;
+      | unit EnvT =>
+          intro ce₂ T₂ H2;
+          cases H2;
+          rfl;
+      | proj EnvT A B n e ce H1 H2 IH =>
+          intro ce₂ T₂ H3;
+          cases H3 with
+          | proj _ a' _ _ _ ce' H4 H5 =>
+              have hA : ce = ce' := by apply IH; apply H4;
+              rw [hA];
+      | lam EnvT A B e ce H IH => 
+          intro ce₂ T₂ H2;
+          cases H2 with
+          | lam _ _ b' _ ce' h =>
+              have hA : ce = ce' := by apply IH; apply h;
+              rw [hA];
+      | box EnvT EnvT₁ A e₁ e₂ ce₁ ce₂ H1 H2 IH1 IH2 => 
+          intro ce' T' H3;
+          cases H3 with
+          | box _ en _ _ _ ce1' ce2' h1 h2 =>
+            have hA : ce₁ = ce1' := by apply IH1; apply h1;
+            have hB : EnvT₁ = en := by apply InferenceUniqueness EnvT EnvT₁ en e₁ ce₁ ce1'; apply H1; apply h1; 
+            have hC : ce₂ = ce2' :=  by apply IH2; rw [hB]; apply h2;
+            rw [hA, hC];
+      | clos EnvT EnvT₁ A B e env ce cenv H1 H2 IH1 IH2 =>
+          intro ce' T' H3;
+          cases H3 with
+          | clos _ et _ bT _ _ ce1' cenv' h1 h2 =>
+            have hA : cenv = cenv' := by apply IH1; apply h1;
+            have hB : EnvT₁ = et := by apply InferenceUniqueness EnvT EnvT₁ et env cenv cenv'; apply H1; apply h1;
+            have hC : ce = ce1' := by apply IH2;  rw [hB]; apply h2; 
+            rw [hA, hC];
+      | app EnvT A B e₁ e₂ ce₁ ce₂ H1 H2 IH1 IH2 =>
+          intro ce' T' H3;
+          cases H3 with
+          | app _ a' _ _ _ ce1' ce2' h1 h2 =>
+            have hA : ce₁ = ce1' := by apply IH1; apply h1;
+            have hB : ce₂ = ce2' := by apply IH2; apply h2;
+            rw [hA, hB];
+      | dmrg EnvT A B e₁ e₂ ce₁ ce₂ H1 H2 IH1 IH2 =>
+          intro ce' T' H3;
+          cases H3 with
+          | dmrg _ a' b' _ _ ce1' ce2' h1 h2 =>
+            have hA : ce₁ = ce1' := by apply IH1; apply h1;
+            have hB : A = a' := by apply InferenceUniqueness EnvT A a' e₁ ce₁ ce1'; apply H1; apply h1;
+            have hC : ce₂ = ce2' := by apply IH2; rw [hB]; apply h2;
+            rw [hA, hC];
+      | ndmrg EnvT A B e₁ e₂ ce₁ ce₂ H1 H2 IH1 IH2 =>
+          intro ce' T' H3;
+          cases H3 with
+          | ndmrg _ a' b' _ _ ce1' ce2' h1 h2 =>
+            have hA : ce₁ = ce1' := by apply IH1; apply h1;
+            have hB : ce₂ = ce2' := by apply IH2; apply h2;
+            rw [hA, hB];
+      | struct EnvT A B e ce H IH => 
+          intro ce' T' H2;
+          cases H2 with
+          | struct _ a' b' _ ce1' h =>
+              have hA : ce = ce1' := by apply IH; apply h;
+              rw [hA];
+      | modapp EnvT A B e₁ e₂ ce₁ ce₂ H1 H2 IH1 IH2 =>
+          intro ce' T' H3;
+          cases H3 with
+          | modapp _ a' _ _ _ ce1' ce2' h1 h2 =>
+            have hA : ce₂ = ce2' := by apply IH2; apply h2;
+            have hB : ce₁ = ce1' := by apply IH1; apply h1;
+            rw [hA, hB];
+      | lrec EnvT A e ce label H IH => 
+          intro ce' T' H2;
+          cases H2 with
+          | lrec _ a' _ ce1' label h =>
+              have hA : ce = ce1' := by apply IH; apply h;
+              rw [hA];
+      | rproj EnvT A B e ce label H1 H2 IH => 
+          intro ce' T' H3;
+          cases H3 with
+          | rproj _ a' b' _ ce1' _ h1 h2 =>
+            have hA : ce = ce1' := by apply IH; apply h1;
+            rw [hA];
+      | slet EnvT A B e₁ e₂ ce₁ ce₂ H1 H2 IH1 IH2 =>
+          intro ce' T' H3;
+          cases H3 with
+          | slet _ _ b' _ _ ce1' ce2' h1 h2 =>
+            have hA : ce₂ = ce2' := by apply IH2; apply h2;
+            have hB : ce₁ = ce1' := by apply IH1; apply h1;
+            rw [hA, hB];
+      | sopen EnvT A B e₁ e₂ ce₁ ce₂ label H1 H2 H3 IH1 IH2 IH3 IH4 =>
+          intro ce' T' H5;
+          cases H5 with
+          | sopen _ a' b' _ _ ce1' ce2' label' h1 h2 h3 h4 =>
+            have hA : ENVCAP.Typ.rcd label A = ENVCAP.Typ.rcd label' a' := by apply InferenceUniqueness EnvT (ENVCAP.Typ.rcd label A) (ENVCAP.Typ.rcd label' a') e₁ ce₁ ce1'; apply H2; apply h2;
+            cases hA;
+            have hB : ce₁ = ce1' := by apply IH2; apply h2;
+            have hC : ce₂ = ce2' := by apply IH4; apply h4;
+            rw [hB, hC];
